src/Std/Tactic/Do/Syntax.lean
@@ -296,7 +296,7 @@ all_goals
 ```
 -/
 macro (name := mspecNoSimp) "mspec_no_simp" spec:(ppSpace colGt term)? : tactic =>
-  `(tactic| ((try with_reducible mspec_no_bind $(mkIdent ``Std.Do.Spec.bind)); mspec_no_bind $[$spec]?))
+  `(tactic| ((try with_reducible mspec_no_bind $(mkIdent ``Std.Do.Spec.bind)) <;> mspec_no_bind $[$spec]?))
 
 syntax "mvcgen_trivial_extensible" : tactic
 
